\subsection{Exercise 3}
\begin{align}
    \Gamma^\lambda_{\mu\nu} &= \frac{1}{2}g^{\lambda\rho} \left(\partial_\mu g_{\nu\rho} + \partial_\nu g_{\rho\mu} - \partial_\rho g_{\mu\nu} \right) \\
    &= \frac{1}{2}g^{\lambda\lambda} \cdot 0 + \frac{1}{2} 0 \cdot \left( \dots \right) \\
    &= 0
\end{align}
\begin{align}
    \Gamma^\lambda_{\mu\mu} &= \frac{1}{2} g^{\lambda\rho} \left(\partial_\mu g_{\mu\rho} + \partial_\mu g_{\rho\mu} - \partial_\rho g_{\mu\mu} \right) \\
    &= - \frac{1}{2} g^{\lambda\lambda} \partial_\lambda g_{\mu\mu} \\
    &= -\frac{1}{2} \left(g_{\lambda\lambda}\right)^{-1} \partial_\lambda g_{\mu\mu}
\end{align}
\begin{align}
    \Gamma^\lambda_{\mu\lambda} &= \frac{1}{2} g^{\lambda\rho} \left(\partial_\mu g_{\lambda\rho} + \partial_\lambda g_{\rho\mu} - \partial_\rho g_{\mu\lambda} \right) \\
    &= \frac{1}{2}g^{\lambda\lambda}\partial_\mu g_{\lambda\lambda} \\
    &= \frac{1}{2 g_{\lambda\lambda}} \partial_\mu g_{\lambda\lambda} \\
    &= \partial_\mu \left(\ln{\sqrt{\left|g_{\lambda\lambda}\right|}}\right)
\end{align}
\begin{align}
    \Gamma^\lambda_{\lambda\lambda} &= \frac{1}{2} g^{\lambda\rho} \left( \partial_\lambda g_{\lambda\rho} + \partial_\lambda g_{\rho\lambda} - \partial_\rho g_{\lambda\lambda} \right) \\
    &= \frac{1}{2g_{\lambda\lambda}} \partial_\lambda g_{\lambda\lambda} \\
    &= \partial_\lambda \left(\ln{\sqrt{\left|g_{\lambda\lambda}\right|}}\right)
\end{align}